git/leanprover/lake/Lake/CLI/Main.lean
@@ -42,18 +42,18 @@ def loadPkg (config : LakeConfig) : LogIO Package := do
 def loadManifestMap (manifestFile : FilePath) : LogIO (Lean.NameMap PackageEntry) := do
   if let Except.ok contents ← IO.FS.readFile manifestFile  |>.toBaseIO then
     match Json.parse contents with
-      | Except.ok json =>
-        match fromJson? json with
-        | Except.ok (manifest : Manifest) =>
-          pure manifest.toMap
-        | Except.error e =>
-          logWarning s!"improperly formatted package manifest: {e}"
-          pure {}
+    | Except.ok json =>
+      match fromJson? json with
+      | Except.ok (manifest : Manifest) =>
+        return manifest.toMap
       | Except.error e =>
-        logWarning s!"invalid JSON in package manifest: {e}"
-        pure {}
+        logWarning s!"improperly formatted package manifest: {e}"
+        return {}
+    | Except.error e =>
+      logWarning s!"invalid JSON in package manifest: {e}"
+      return {}
   else
-    pure {}
+    return {}
 
 def loadWorkspace (config : LakeConfig) (updateDeps := false) : LogIO Workspace := do
   let pkg ← loadPkg config
@@ -228,8 +228,9 @@ def serve (config : LakeConfig) (args : Array String) : LogIO UInt32 := do
       let ctx := mkLakeContext ws config
       pure (← LakeT.run ctx getAugmentedEnv, ws.root.moreServerArgs)
     catch _ =>
+      let installEnv := mkInstallEnv config.leanInstall config.lakeInstall
       logWarning "package configuration has errors, falling back to plain `lean --server`"
-      pure (#[(invalidConfigEnvVar, "1")], #[])
+      pure (installEnv.push (invalidConfigEnvVar, "1"), #[])
   (← IO.Process.spawn {
     cmd := config.leanInstall.lean.toString
     args := #["--server"] ++ moreServerArgs ++ args
